

SDS 387 Linear Models

Fall 2025

Lecture 19 - Tue, Nov 4, 2025

Instructor: Prof. Ale Rinaldo

OLS ESTIMATOR IN FIXED-DESIGN SETTING

Today we will assume

$$y_i = \Phi_i^T \beta^* + \varepsilon_i \quad \text{where } \varepsilon_1, \dots, \varepsilon_n \stackrel{\text{i.i.d.}}{\sim} (0, \sigma^2)$$

$i = 1, \dots, n$

and

Φ_1, \dots, Φ_n are fixed (deterministic)
vectors in \mathbb{R}^d

↓

2 assumptions i) linearity

$$\mathbb{E}[y_i] = \Phi_i^T \beta^*$$

(Aside, if the Φ_i 's were random

linearity means $\mathbb{E}[y_i | \Phi_i] = \Phi_i^T \beta^*$)

ii) fixed covariates

- The fixed covariates assumption is unrealistic but you can assume that we are conditioning on the Φ_i 's.

- When the model is linear and the covariates are random (i.e. $\mathbb{E}[Y_i | \Phi_i] = \Phi_i^T \beta^*$) the distribution of the covariates (hence the covariates themselves) is ancillary. So it is natural to condition on the Φ_i 's. This is only true if linearity holds (otherwise we know that the projection parameter $\beta^* = \mathbb{E}[\Phi_i \Phi_i^T]^{-1} \mathbb{E}[Y_i \Phi_i]$ depends on the distribution of the covariates).

See

Boja et al. (2019)

- Remark: If $\varepsilon_1, \dots, \varepsilon_n \stackrel{iid}{\sim} N(0, \sigma^2)$ then the likelihood of the data Y_1, \dots, Y_n is

$$\left(\frac{1}{\sqrt{2\pi} \sigma} \right)^n \exp \left\{ - \frac{\|Y - \Phi \beta^*\|^2}{2\sigma^2} \right\}$$

and the OLS $\hat{\beta}$ is the MLE of β^* .

- Now, for any $\beta \in \mathbb{R}^d$, the risk of β is

$$R(\beta) = \mathbb{E}_Y \left[\frac{\|Y - \Phi \beta\|^2}{n} \right] = \mathbb{E}_\varepsilon \left[\frac{\| \Phi (\beta^* - \beta) + \varepsilon \|^2}{n} \right]$$

vector in \mathbb{R}^n
of errors
 $\varepsilon = \begin{bmatrix} \varepsilon_1 \\ \vdots \\ \varepsilon_n \end{bmatrix}$

$$= (\beta^* - \beta)^T \underbrace{\frac{\Phi^T \Phi}{n}}_{\text{}} (\beta^* - \beta) + \mathbb{E}_\varepsilon \left[\frac{\|\varepsilon\|^2}{n} \right]$$

$$\frac{1}{n} \sum_{i=1}^n \Phi_i \Phi_i^T$$

$$= (\beta^* - \beta)^T \hat{\Sigma} (\beta^* - \beta) + \sigma^2$$

$$= \|\beta^* - \beta\|_{\Sigma}^2 + \sigma^2$$

↓

$$R(\beta^*)$$

↓

The quantity $R(\beta) - R(\beta^*) \geq 0$ is the **excess risk**

• Remark: You can think of $R(\beta)$ as $\mathbb{E}_{Y|\Phi} \left[\frac{\|Y - \Phi\beta\|^2}{n} \mid \Phi \right]$ if Φ were random (assuming linearity).

• So let's analyze $R(\hat{\beta}) - R(\beta^*)$, the excess risk of the OLS $\hat{\beta}$. Note this excess risk is a random variable! Let's compute its expectation:

• Remark: think of $R(\hat{\beta})$ as $\mathbb{E}_{Y_{\text{new}}} \left[\frac{\|Y_{\text{new}} - \Phi\hat{\beta}\|^2}{n} \right]$ where $Y_{\text{new}} \in \mathbb{R}^n$ is a new draw of data independent of the observations.

$$\mathbb{E}[R(\hat{\beta})] - R(\beta^*) = \mathbb{E}_{\hat{\beta}} \left[(\beta^* - \hat{\beta})^T \hat{\Sigma} (\beta^* - \hat{\beta}) \right]$$

$\|\beta^* - \hat{\beta}\|_{\hat{\Sigma}}^2 = \|\beta^* - \mathbb{E}[\hat{\beta}] + \mathbb{E}[\hat{\beta}] - \hat{\beta}\|_{\hat{\Sigma}}^2$
 $= \dots$

= add (subtract $\mathbb{E}[\hat{\beta}]$)

Exercise!

$$= \mathbb{E} \left[\|\hat{\beta} - \mathbb{E}[\hat{\beta}]\|_{\hat{\Sigma}}^2 \right] + \|\beta^* - \mathbb{E}[\hat{\beta}]\|_{\hat{\Sigma}}^2$$

↓
variance term for $\hat{\beta}$
bias term

$$\mathbb{E} \left[(\hat{\beta} - \mathbb{E}[\hat{\beta}])^T \hat{\Sigma} (\hat{\beta} - \mathbb{E}[\hat{\beta}]) \right] = \mathbb{E} \left[\text{tr} \left(\hat{\Sigma} (\hat{\beta} - \mathbb{E}[\hat{\beta}]) (\hat{\beta} - \mathbb{E}[\hat{\beta}])^T \right) \right] \quad (3)$$

$$= \text{tr} \left(\hat{\Sigma} \underbrace{\mathbb{E}[(\hat{\beta} - \mathbb{E}[\hat{\beta}])(\hat{\beta} - \mathbb{E}[\hat{\beta}])^T]}_{\text{Var}[\hat{\beta}]} \right)$$

Next, let's evaluate the variance and bias of $\hat{\beta}$:

bias : $\mathbb{E}[\hat{\beta}] = (\Phi^T \Phi)^{-1} \Phi^T \underbrace{\mathbb{E}[Y]}_{\Phi \beta^*} = \beta^*$ because $\hat{\Sigma}$ is invertible

↓
no bias

This derivation is valid also when Φ is random:

$$\mathbb{E}[\hat{\beta}] = \mathbb{E}[\underbrace{\mathbb{E}[\hat{\beta} | \Phi]}_{\beta^*}] = \beta^*$$

↓
Linearity here is crucial.

variance

$$\begin{aligned} \text{Var}[\hat{\beta}] &= \text{Var}[(\Phi^T \Phi)^{-1} \Phi^T Y] \\ &= (\Phi^T \Phi)^{-1} \Phi^T \underbrace{\text{Var}[Y]}_{\sigma^2 I_n} \Phi (\Phi^T \Phi)^{-1} \\ &= \sigma^2 (\Phi^T \Phi)^{-1} \end{aligned}$$

var[AY] = A var[Y] A^T

So we can now plug-in these expressions and get

$$\mathbb{E}[R(\hat{\beta})] - R(\beta^*) = \sigma^2 \frac{d}{n}$$

PA/ We only need to evaluate

$$\begin{aligned}
\mathbb{E} \left[\|\hat{\beta} - \underbrace{\mathbb{E}[\hat{\beta}]}_{\beta^*} \|_{\hat{\Sigma}}^2 \right] &= \mathbb{E} \left[\|\cancel{\beta^*} + (\Phi^T \Phi)^{-1} \Phi^T \varepsilon - \cancel{\beta^*} \|_{\hat{\Sigma}}^2 \right] \\
(\Phi^T \Phi)^{-1} \Phi^T (\Phi \beta^* + \varepsilon) &= \mathbb{E} \left[\left\| \hat{\Sigma}^{-1} \frac{\Phi^T \varepsilon}{n} \right\|_{\hat{\Sigma}}^2 \right] \\
&= \mathbb{E} \left[\varepsilon^T \frac{\Phi}{n} \hat{\Sigma}^{-1} \cancel{\hat{\Sigma}} \cancel{\hat{\Sigma}^{-1}} \frac{\Phi^T \varepsilon}{n} \right] \\
&= \frac{1}{n} \mathbb{E} \left[\varepsilon^T \underbrace{\Phi (\Phi^T \Phi)^{-1} \Phi^T}_{H \text{ the hat matrix}} \varepsilon \right] \\
&= \frac{1}{n} \mathbb{E} \left[\varepsilon^T H \varepsilon \right] \\
&= \frac{1}{n} \mathbb{E} \left[\text{tr}(H \varepsilon \varepsilon^T) \right] \\
&= \frac{1}{n} \text{tr} \left(H \underbrace{\mathbb{E}[\varepsilon \varepsilon^T]}_{\sigma^2 I_n} \right) \\
&= \frac{\sigma^2}{n} \text{tr}(H) \\
&= \sigma^2 \frac{d}{n}
\end{aligned}$$

Other proof:

$$\begin{aligned}
\mathbb{E} \left[\underbrace{\|\hat{\beta} - \beta^*\|_{\hat{\Sigma}}^2}_{\mathbb{E}[\hat{\beta}]} \right] &= \mathbb{E} \left[\text{tr} \left(\hat{\Sigma}^{-1} (\hat{\beta} - \beta^*) (\hat{\beta} - \beta^*)^T \right) \right] \\
&= \text{tr} \left(\hat{\Sigma}^{-1} \text{Var}[\hat{\beta}] \right) \\
&= \text{tr} \left(\hat{\Sigma}^{-1} \frac{\sigma^2}{n} \hat{\Sigma} \right) \\
&= \frac{\sigma^2}{n} \text{tr}(I_d) = \sigma^2 \frac{d}{n}
\end{aligned}$$

Remarks:

i) The $\sigma^2 \frac{d}{n}$ bound for the excess risk of $\hat{\beta}$ (OLS) is optimal, in a minimax sense

ii) More refined analysis will give you high prob. bounds for excess risk.

iii) Recall that this result tells that

$$\mathbb{E} [R(\hat{\beta})] = \mathbb{E}_{y_{\text{new}}, Y} \left[\frac{\|y_{\text{new}} - \Phi \hat{\beta}\|^2}{n} \right]$$

$$\downarrow = \sigma^2 \left(1 + \frac{d}{n} \right)$$

this is called the out-of-sample risk

What if we used the in-sample expected risk?

$$\mathbb{E} [\hat{R}(\hat{\beta})] = \mathbb{E}_Y \left[\frac{\|Y - \Phi \hat{\beta}\|^2}{n} \right] = \sigma^2 \left(1 - \frac{d}{n} \right)$$

\downarrow FW

Wrong measure of risk! The risk is at least $R(\beta^*) = \sigma^2$
while $\mathbb{E} [\hat{R}(\hat{\beta})] < \sigma^2$